Start looking at new definition of calls with ghost state
The new version keeps track of which locs it has _not_ added to the code
table, because the relevant function body contained free variables. The
hope is that correctness for this version will be easier because we can
refer to the discarded locs. Although, maybe it would also be possible
to consider the difference between the locs in the expression and the
ones picked up by the original calls function...?

compiler/backend/proofs/clos_callProofScript.sml
@@ -27,6 +27,18 @@ val v_size_lemma = prove(
   ``MEM (v:closSem$v) vl ⇒ v_size v < v1_size vl``,
   Induct_on `vl` >> dsimp[v_size_def] >> rpt strip_tac >>
   res_tac >> simp[]);
+
+val list_to_num_set_append = Q.store_thm("list_to_num_set_append",
+  `∀l1 l2. list_to_num_set (l1 ++ l2) = union (list_to_num_set l1) (list_to_num_set l2)`,
+  Induct \\ rw[list_to_num_set_def]
+  \\ rw[Once insert_union]
+  \\ rw[Once insert_union,SimpRHS]
+  \\ rw[union_assoc])
+
+val subspt_domain_SUBSET = Q.store_thm("subspt_domain_SUBSET",
+  `subspt s1 s2 ⇒ domain s1 ⊆ domain s2`,
+  rw[subspt_def,SUBSET_DEF]);
+
 (* -- *)
 
 val subg_def = Define`
@@ -198,6 +210,14 @@ val domain_FST_insert_each = Q.store_thm("domain_FST_insert_each",
   \\ rw[insert_each_def,GENLIST_CONS,o_DEF,ADD1,LEFT_ADD_DISTRIB]
   \\ simp[EXTENSION,MEM_GENLIST]
   \\ metis_tac[ADD_ASSOC,ADD_COMM]);
+
+val SND_code_list_change = Q.store_thm("SND_code_list_change",
+  `∀loc fns g g'. SND g = SND g' ⇒
+    SND (code_list loc fns g) = SND (code_list loc fns g')`,
+  ho_match_mp_tac code_list_ind
+  \\ rw[code_list_def]
+  \\ Cases_on`g'` \\ rw[code_list_def]
+  \\ fs[FORALL_PROD]);
 
 val MAP_FST_code_list = Q.store_thm("MAP_FST_code_list",
   `∀loc fns g.
@@ -438,6 +458,182 @@ val closed_Fn = Q.store_thm("closed_Fn",
   \\ Cases_on`lookup (args+n) (db_to_set l)` \\ rw[]
   \\ Cases_on `x` \\ fs[GSYM lookup_db_to_set]
   \\ res_tac \\ fs[]);
+
+(* alternative definition of calls which tracks more information *)
+
+val exp_size_def = closLangTheory.exp_size_def;
+val exp1_size_lemma = closLangTheory.exp1_size_lemma;
+val EL_MEM_LEMMA = prove(
+  ``!xs i x. i < LENGTH xs /\ (x = EL i xs) ==> MEM x xs``,
+  Induct \\ fs [] \\ REPEAT STRIP_TAC \\ Cases_on `i` \\ fs []);
+val exp3_size_MAP_SND = prove(
+  ``!fns. exp3_size (MAP SND fns) <= exp1_size fns``,
+  Induct \\ fs [exp_size_def,FORALL_PROD]);
+val calls2_def = tDefine "calls2" `
+  (calls2 [] g = ([],g)) /\
+  (calls2 ((x:closLang$exp)::y::xs) g =
+     let (e1,g) = calls2 [x] g in
+     let (e2,g) = calls2 (y::xs) g in
+       (e1 ++ e2,g)) /\
+  (calls2 [Var v] g =
+     ([Var v],g)) /\
+  (calls2 [If x1 x2 x3] g =
+     let (e1,g) = calls2 [x1] g in
+     let (e2,g) = calls2 [x2] g in
+     let (e3,g) = calls2 [x3] g in
+     let e1 = HD e1 in
+     let e2 = HD e2 in
+     let e3 = HD e3 in
+       ([If e1 e2 e3],g)) /\
+  (calls2 [Let xs x2] g =
+     let (e1,g) = calls2 xs g in
+     let (e2,g) = calls2 [x2] g in
+     let e2 = HD e2 in
+       ([Let e1 e2],g)) /\
+  (calls2 [Raise x1] g =
+     let (e1,g) = calls2 [x1] g in
+     let e1 = HD e1 in
+       ([Raise e1],g)) /\
+  (calls2 [Tick x1] g =
+     let (e1,g) = calls2 [x1] g in
+     let e1 = HD e1 in
+       ([Tick e1],g)) /\
+  (calls2 [Handle x1 x2] g =
+     let (e1,g) = calls2 [x1] g in
+     let (e2,g) = calls2 [x2] g in
+     let e1 = HD e1 in
+     let e2 = HD e2 in
+       ([Handle e1 e2],g)) /\
+  (calls2 [Call dest xs] g =
+     let (xs,g) = calls2 xs g in
+       ([Call dest xs],g)) /\
+  (calls2 [Op op xs] g =
+     let (e1,g) = calls2 xs g in
+       ([Op op e1],g)) /\
+  (calls2 [App loc_opt x xs] g =
+     let (es,g) = calls2 xs g in
+     let (e1,g) = calls2 [x] g in
+     let e1 = HD e1 in
+     let loc = (case loc_opt of SOME loc => loc | NONE => 0) in
+       if IS_SOME loc_opt /\ loc ∈ (FST (FST g)) then
+         if pure x then ([Call (loc+1) es],g) else
+           ([Let (SNOC e1 es)
+              (Call (loc+1) (GENLIST Var (LENGTH es)))],g)
+       else ([App loc_opt e1 es],g)) /\
+  (calls2 [Fn loc_opt ws num_args x1] g =
+     let loc = (case loc_opt of SOME loc => loc | NONE => 0) in
+     let new_g = ((loc INSERT (FST (FST g)),SND(FST g)),SND g) in
+     let (e1,new_g) = calls2 [x1] new_g in
+     let new_g = (FST new_g,(loc+1,num_args,HD e1)::SND new_g) in
+       if closed (Fn loc_opt ws num_args (HD e1)) then
+         ([Fn loc_opt ws num_args
+             (Call (loc+1) (GENLIST Var num_args))],new_g)
+       else
+         let g = ((FST(FST g),(loc INSERT (SND (FST g)))),SND g) in
+         let (e1,g) = calls2 [x1] g in
+           ([Fn loc_opt ws num_args (HD e1)],g)) /\
+  (calls2 [Letrec loc_opt ws fns x1] g =
+     let loc = (case loc_opt of SOME loc => loc | NONE => 0) in
+     let new_g = ((set (GENLIST (λi. 2*i+loc) (LENGTH fns)) ∪ (FST(FST g)),SND (FST g)), SND g) in
+     let (fns1,new_g) = calls2 (MAP SND fns) new_g in
+       if EVERY2 (\(n,_) p. closed (Fn NONE NONE n p)) fns fns1 then
+         let new_g = code_list loc (ZIP (MAP FST fns,fns1)) new_g in
+         let (e1,g) = calls2 [x1] new_g in
+           ([Letrec loc_opt ws (calls_list loc fns) (HD e1)],new_g)
+       else
+         let g = ((FST(FST g),(set (GENLIST (λi. 2*i+loc) (LENGTH fns)) ∪ (SND (FST g)))),SND g) in
+         let (fns1,g) = calls2 (MAP SND fns) g in
+         let (e1,g) = calls2 [x1] g in
+           ([Letrec loc_opt ws (ZIP (MAP FST fns,fns1)) (HD e1)],g))`
+ (WF_REL_TAC `measure (exp3_size o FST)`
+  \\ REPEAT STRIP_TAC
+  \\ fs [GSYM NOT_LESS]
+  \\ IMP_RES_TAC EL_MEM_LEMMA
+  \\ IMP_RES_TAC exp1_size_lemma
+  \\ assume_tac (SPEC_ALL exp3_size_MAP_SND)
+  \\ DECIDE_TAC);
+
+val calls2_ind = theorem"calls2_ind";
+
+val calls_calls2 = Q.store_thm("calls_calls2",
+  `∀xs g0 ys g g02.
+    calls xs g0 = (ys,g)
+    ⇒
+    (*let g2 = set (code_locs xs) DIFF (domain (FST g) DIFF domain (FST g0)) in *)
+    ∃g2.
+    calls2 xs ((domain(FST g0),g02),SND g0) = (ys,((domain (FST g), g2),SND g))(* ∧
+    DISJOINT g02 g2 ∧
+    DISJOINT g2 (domain (FST g) DIFF domain (FST g0)) *)`,
+  ho_match_mp_tac calls_ind
+  \\ rw[calls_def,calls2_def,code_locs_def]
+  \\ rpt(pairarg_tac \\ fs[]) \\ rveq
+  \\ TRY (
+    first_x_assum(qspec_then`g02`mp_tac)\\rw[]
+    \\ first_x_assum(qspec_then`g2`mp_tac)\\rw[]
+    \\ first_x_assum(qspec_then`g2'`mp_tac)\\rw[])
+  \\ every_case_tac \\ fs[] \\ rw[]
+  \\ TRY (
+    first_x_assum(qspec_then`g02`mp_tac)\\rw[]
+    \\ first_x_assum(qspec_then`g2`mp_tac)\\rw[]
+    \\ NO_TAC)
+  \\ TRY (
+    fs[domain_FST_insert_each,GSYM INSERT_SING_UNION]
+    \\ first_x_assum(qspec_then`g02`mp_tac)\\rw[]
+    \\ spose_not_then strip_assume_tac \\ fs[] \\ rw[]
+    \\ first_x_assum(qspec_then`g2`mp_tac)\\rw[]
+    \\ spose_not_then strip_assume_tac \\ fs[] \\ rw[]
+    \\ fs[domain_lookup] \\ rfs[IS_SOME_EXISTS]
+    \\ NO_TAC)
+  \\ TRY (
+    first_x_assum(qspec_then`0 INSERT g02`mp_tac) \\ rw[]
+    \\ fs[domain_FST_insert_each,GSYM INSERT_SING_UNION]
+    \\ first_x_assum(qspec_then`g02`mp_tac) \\ rw[]
+    \\ fs[] \\ NO_TAC)
+  \\ TRY (
+    first_x_assum(qspec_then`x INSERT g02`mp_tac) \\ rw[]
+    \\ fs[domain_FST_insert_each,GSYM INSERT_SING_UNION]
+    \\ first_x_assum(qspec_then`g02`mp_tac) \\ rw[]
+    \\ fs[] \\ NO_TAC)
+  \\ TRY (
+    fs[domain_FST_insert_each]
+    \\ last_x_assum(qspec_then`g02`mp_tac) \\ rw[]
+    \\ qpat_assum`calls2 _ (code_list _ _ _) = _`mp_tac
+    \\ CONV_TAC(LAND_CONV(LAND_CONV(RAND_CONV(REWR_CONV (GSYM PAIR)))))
+    \\ PURE_REWRITE_TAC[FST_code_list]
+    \\ simp[]
+    \\ qmatch_goalsub_abbrev_tac`code_list ll ff (g1,SND gg)`
+    \\ qispl_then[`ll`,`ff`,`(g1,SND gg)`,`gg`]mp_tac SND_code_list_change
+    \\ simp[] \\ disch_then kall_tac \\ unabbrev_all_tac
+    \\ first_x_assum(qspec_then`g2`mp_tac)\\rw[] \\ fs[]
+    \\ CONV_TAC(QUANT_CONV(LAND_CONV(REWR_CONV(GSYM PAIR))))
+    \\ PURE_REWRITE_TAC[FST_code_list]
+    \\ simp[]
+    \\ match_mp_tac SND_code_list_change
+    \\ simp[] )
+  \\ TRY (
+   fs[domain_FST_insert_each]
+   \\ first_x_assum(qspec_then`g02`mp_tac) \\ rw[]
+   \\ qmatch_asmsub_abbrev_tac`g01 ∪ g02`
+   \\ first_x_assum(qspec_then`g01 ∪ g02`mp_tac)
+   \\ rw[]
+   \\ first_x_assum(qspec_then`g2'`mp_tac) \\ rw[] ));
+
+(*
+val calls2_disjoint = Q.store_thm("calls2_disjoint",
+  `∀xs g0 ys g.
+    calls2 xs g0 = (ys,g) ∧
+    DISJOINT (FST (FST g0)) (SND (FST g0)) ∧
+    every_Fn_SOME xs ∧
+    DISJOINT (FST (FST g0)) (set (code_locs xs)) ∧
+    DISJOINT (SND (FST g0)) (set (code_locs xs))
+    ⇒
+    DISJOINT (FST (FST g)) (SND (FST g))`,
+  ho_match_mp_tac calls2_ind
+  \\ rw[calls2_def] \\ fs[code_locs_def]
+  \\ rpt(pairarg_tac \\ fs[])
+  \\ every_case_tac \\ fs[] \\ rw[]
+  \\ first_x_assum match_mp_tac
+*)
 
 (* compiler correctness *)
 
